wip

Http/Ssl/Handshake.lean
@@ -1,3 +1,6 @@
+import Std.Data.List.Lemmas
+import Std.Data.Nat.Lemmas
+
 namespace Ssl
 
 -- Use RFC 8446 as base
@@ -24,17 +27,46 @@ def concatMap (f : α → Array β) (as : List α) : Array β :=
 def Vector.toBytes [ToBytes α] : Vector α n → Array UInt8
   | ⟨ as , _ ⟩ => (concatMap (fun a : α => (@ToBytes.toBytes α) a) as)
 
--- def Vector.fromBytes [FromBytes α p] : Vector UInt8 (m * p) → Except String (Vector α m) := fun arr =>
---   match m with
---   | .zero => .ok ⟨ [], _ ⟩
---   | (.succ m) =>
---     match (FromBytes.fromBytes ⟨ ⟩).toArray, by {
---       simp
-      
---     }⟩ : Except String α) with
---     | .ok a => _
---     | .error s => .error s
+def ineq_lemma (n p : Nat) : p ≤ (.succ n) * p := by
+  induction p with
+  | zero => simp
+  | succ p' ihp => {
+    rw [Nat.mul_succ, ← Nat.add_one]
+    exact Nat.add_le_add ihp (Nat.pos_of_ne_zero (by simp))
+  }
 
+def nat_lemma : Nat.succ m * p - p = m * p := by 
+  induction p with
+  | zero => simp
+  | succ p' ihp => {
+    rw [Nat.mul_succ, Nat.succ_mul, Nat.mul_succ, ← ihp]
+    
+  }
+
+
+def Vector.take (h : n ≤ m) (as : Vector α m) : Vector α n :=
+  let ⟨ asl , aslh ⟩ := as
+  let taken := asl.take n
+  ⟨ taken , List.length_take_of_le (aslh ▸ h)⟩
+
+theorem length_drop_of_le (h : n ≤ List.length l) : List.length (.drop n l) = List.length l - n := by simp
+
+def Vector.drop (h : n ≤ m) (as : Vector α m) : Vector α (m - n) :=
+  let ⟨ asl , aslh ⟩ := as
+  let taken := asl.drop n
+  ⟨ taken , aslh ▸ length_drop_of_le (aslh ▸ h)⟩
+
+def Vector.fromBytes [FromBytes α p] : Vector UInt8 (m * p) → Except String (Vector α m) := fun as =>
+  match m with
+  | .zero => .ok ⟨ [], (by simp) ⟩
+  | (.succ m) => 
+    match ((FromBytes.fromBytes (Vector.take (ineq_lemma _ _) as)) : Except String α) with
+    | .ok a => 
+      match Vector.fromBytes (Vector.drop (ineq_lemma _ _) as) with
+      | .ok ⟨ as , ash ⟩ => Except.ok (⟨a :: as, ash ▸ List.length_cons a as⟩ )
+      | .error e => Except.error e
+    | .error e => Except.error e
+  
 instance [ToBytes α] : ToBytes (Vector α n) where
   toBytes := fun v => Vector.toBytes v
 
@@ -45,9 +77,7 @@ def VariableVector.toBytes [ToBytes α] : VariableVector α l u → Array UInt8
   | ⟨ arr , _ ⟩ => 
   arr.concatMap (fun a : α => (@ToBytes.toBytes α) a)
 
-structure Random where
-  gmxUnixTime : UInt32
-  randomBytes : Vector UInt8 28
+abbrev Random := Vector UInt8 28
 
 def UInt8.toBytes : UInt8 → Array UInt8 := fun i => #[i]
 
@@ -63,33 +93,49 @@ def UInt32.toBytes : UInt32 → Array UInt8 :=
 instance : ToBytes UInt32 where
   toBytes := UInt32.toBytes
 
-def Random.toBytes : Random → Array UInt8 :=
-  fun r => ToBytes.toBytes (gmxUnixTime r) ++ (randomBytes r).val
-
 
 abbrev SessionId := VariableVector UInt8 0 32
 
 abbrev CipherSuite := Vector UInt8 2
+
+inductive ExtensionType where
+  | serverName | maxFragmentLength | statusRequest | supportedGroups | signatureAlgoritms | useSrtp
+  | heartbeat | applicationLayerProtocolNegotiation | signedCertificateTimestamp
+  | clientCertificateType | serverCertificateType | padding | preSharedKey
+  | earlyData | supportedVersions | cookie | pskKeyExchangeModes | certificateAuthorities
+  | oidFilters | postHandshakeAuth | signatureAlgorithmsCert | keyShare
+
+structure Extension where
+  extensionType : ExtensionType
+  extensionData : VariableVector UInt8 0 (2^16-1)
  
 
 structure ClientHello where
   protocolVersion : ProtocolVersion
   random : Random
   cipherSuites : VariableVector CipherSuite 2 (2^16-1)
-  -- extensions : to be implemented
+  extensions : VariableVector Extension 8 (2^16-1)
 
--- v1.2 hardcoded
+
 def ClientHello.toBytes : ClientHello → Array UInt8 := fun ch =>
-  #[0x03, 0x03] ++ ch.random.toBytes ++ #[0] ++ ch.cipherSuites.toBytes ++ #[0]
-   -- Empty extensions
-   ++ #[0 , 0]
+  -- v1.2 hardcoded
+  #[0x03, 0x03] 
+    ++ ch.random.toBytes 
+    -- Legacy session id
+    ++ #[0] 
+    ++ ch.cipherSuites.toBytes 
+    -- Legacy Compression methods
+    ++ #[0]
+    -- Empty extensions
+    ++ #[0 , 0]
 
 structure ServerHello where
   serverVersion : ProtocolVersion
   random : Random
-  sessionId : SessionId
+  -- legacySessionIdEcho : SessionId (not relevant, since we don't send sessionIds)
   cipherSuite : CipherSuite
-  compressionMethod : CompressionMethod
+  -- compressionMethod : CompressionMethod
+  extensions : VariableVector Extension 6 (2^16-1)
 
 def HandshakeType.asType : HandshakeType → Type
   | .clientHello => ClientHello
